src/verified_adapter.mli
@@ -4,12 +4,17 @@ open Relation
 open Helper
 
 val is_monitorable: Db.schema -> formula -> bool * (formula * string) option
-val convert_formula: Db.schema -> formula -> Verified.Monitor.formula
+val convert_formula: Db.schema -> int -> formula -> Verified.Monitor.tysym Verified.Monitor.formula
 
 type db
 val empty_db: db
 val insert_into_db: Table.schema -> string list -> db -> db
 
+type tyssig 
+val convert_into_tysym: tcst -> Verified.Monitor.tysym
+val convert_schema_into_sig: Db.schema -> tyssig
+val type_check_formula: Db.schema -> Verified.Monitor.tysym Verified.Monitor.formula -> Verified.Monitor.ty Verified.Monitor.formula option
+
 type state
-val init: Verified.Monitor.formula -> state
+val init: Verified.Monitor.ty Verified.Monitor.formula -> state
 val step: MFOTL.timestamp -> db -> state -> (int * MFOTL.timestamp * relation) list * state
